Veir/Analysis.lean
@@ -1,8 +1,10 @@
 module
 
 public import Veir.Analysis.DataFlowFramework
+public import Veir.Analysis.DataFlow.MonotoneFramework
 public import Veir.Analysis.DataFlow.DominanceAnalysis
 public import Veir.Analysis.DataFlow.DeadCodeAnalysis
 public import Veir.Analysis.DataFlow.SparseAnalysis
 public import Veir.Analysis.DataFlow.SparseConstantPropagationAnalysis
+public import Veir.Analysis.DataFlow.Soundness
 
